c_stubs/tls13_pulse_shims.c
@@ -1,5 +1,6 @@
 #define TLS13_PULSE_SHIMS_IMPLEMENTATION
 #include "tls13_crypto_external.h"
+#include "krmllib.h"
 
 #include <string.h>
 
@@ -26,4 +27,12 @@ void Pulse_Lib_Array_memcpy_l(
     void *dst_bytes,
     void *squash) {
   Pulse_Lib_Array_memcpy(len, src, dst, src_bytes, dst_bytes, squash);
+}
+
+krml_checked_int_t Prims_op_Subtraction(krml_checked_int_t x, krml_checked_int_t y) {
+  return x - y;
+}
+
+bool Prims_op_LessThan(krml_checked_int_t x0, krml_checked_int_t x1) {
+  return x0 < x1;
 }
